some work on Hoare logic for entire executable programs (based on small step semantics)

Hoare/Multistep_Hoare.thy
@@ -46,13 +46,186 @@ definition VTSMx ::
    ('mstate \<Rightarrow> bool) \<Rightarrow>
    ('x gensyn) \<Rightarrow>
    ('mstate \<Rightarrow> bool) \<Rightarrow>
-   bool" where
+   bool"
+  (" |! _ !| !% {!_!} _ {!_!}")  
+  where
 "VTSMx gs P x Q =
   (\<forall> m m' n . 
     P m \<longrightarrow>
     gensyn_sem_small_exec_many gs x n m = (m', Halt) \<longrightarrow>
     Q m')"
 
+lemma VTSMI :
+  assumes
+    "\<And> m m' n .
+      P m \<Longrightarrow>
+      gensyn_sem_small_exec_many gs x n m = (m', Halt) \<Longrightarrow> Q m'"
+  shows "|! gs !| !% {!P!} x {!Q!}" using assms
+  by(auto simp add: VTSMx_def)
+
+lemma VTSME :
+  assumes H : "|! gs !| !% {!P!} x {!Q!}"
+  assumes H1 : "P m"
+  assumes H2 : "gensyn_sem_small_exec_many gs x n m = (m', Halt)"
+  shows "Q m'" using assms
+  by(auto simp add: VTSMx_def)
+
+lemma semprop2I :
+  "(!f) a1 a2 (f a1 a2)"
+  by(auto simp add: semprop2_def)
+
+lemma semprop2E :
+  assumes H : "(!f) a1 a2 a3"
+  shows "a3 = f a1 a2" using assms
+  by(auto simp add: semprop2_def)
+
+(* lifting Hoare rules from single step into VTSM *)
+
+lemma vtsm_lift_halt :
+  assumes H0 : "gs_sem f' = f"
+  assumes Hstart : "\<And> st . P st \<Longrightarrow> gs_getpath f' st = Some p"
+  assumes Hend : "\<And> st . Q st \<Longrightarrow> gs_getpath f' st = None"
+  assumes Hp : "gensyn_get prog p = Some (G s l)"
+  assumes H : "(!f) % {{P}} s {{Q}}"
+  shows "|! f' !| !% {!P!} prog {!Q!}" using assms
+  
+  apply(cases f'; auto simp add: VTSMx_def VT_def)
+  apply(case_tac n; auto split: option.splits)
+  apply(drule_tac x = m in spec) apply(auto)
+  apply(drule_tac x = "f s m" in spec)
+  apply(case_tac nat; auto simp add: semprop2_def split:option.splits)
+  done
+
+(* not totally sure this is true though.
+   plus even if it is it's probably going to be annoying to reason with *)
+lemma vtsm_lift_halt_p :
+  assumes H0 : "gs_sem f' = f"
+  assumes Hp : "gensyn_get prog p = Some (G s l)"
+  assumes H : "(!f) % {{P}} s {{Q}}"
+  assumes H' : "(!f) % {{(\<lambda> st . gs_getpath f' st = Some p)}} s
+                       {{(\<lambda> st . gs_getpath f' st = None)}}"
+  shows "|! f' !| !% {! (\<lambda> st . P st \<and> gs_getpath f' st = Some p) !} prog 
+                     {! (\<lambda> st . Q st \<and> gs_getpath f' st = None) !}" 
+proof-
+  have Combine :
+    "(! gs_sem f') % {{\<lambda>st. P st \<and> gs_getpath f' st = Some p}} s {{\<lambda>st. Q st \<and> gs_getpath f' st = None}}"
+    using Hoare.VandI[OF H H'] unfolding H0
+    by auto
+  show "|! f' !| !% {!\<lambda>st. P st \<and>
+                         gs_getpath f' st =
+                         Some p!} prog {!\<lambda>st. Q st \<and> gs_getpath f' st = None!}"
+
+  using vtsm_lift_halt[OF H0, of "(\<lambda> st . P st \<and> gs_getpath f' st = Some p)" p
+                                 "(\<lambda> st . Q st \<and> gs_getpath f' st = None)",
+                       OF _ _ Hp]
+  using Combine unfolding H0
+  by(auto)
+qed
+
+lemma vtsm_lift_cont :
+  assumes H0 : "gs_sem f' = f"
+  assumes Hstart : "\<And> st . P st \<Longrightarrow> gs_getpath f' st = Some p" 
+(*  assumes Hend : "\<And> st . Q st \<Longrightarrow> gs_getpath f' st = Some p'" *)
+  assumes Hp : "gensyn_get prog p = Some (G s l)"
+  assumes H : "(!f) % {{P}} s {{Q}}"
+  assumes H' : "|! f' !| !% {!Q!} prog {!Q'!}"
+  shows "|! f' !| !% {!P!} prog {!Q'!}" using assms
+  apply(cases f'; auto simp add: VTSMx_def VT_def)
+  apply(drule_tac x = m in spec) apply(auto)
+  apply(case_tac n; auto)
+  apply(drule_tac x = "f s m" in spec) apply(auto simp add: semprop2_def)
+  done
+
+lemma vtsm_lift_cont_p :
+  assumes H0 : "gs_sem f' = f"
+  assumes Hp : "gensyn_get prog p = Some (G s l)"
+  assumes H : "(!f) % {{P}} s {{Q}}"
+  assumes Hrec : "|! f' !| !% {!Q!} prog {!Q'!}"
+  shows "|! f' !| !% {!(\<lambda> st . P st \<and> gs_getpath f' st = Some p)!} prog {!Q'!}" using assms
+proof-
+
+  have H' : "(!f) % {{(\<lambda>  st . gs_getpath f' st = Some p)}} s {{(\<lambda> st.  True)}}"
+    unfolding VT_def by auto
+
+  have Combine:
+    "(! gs_sem f') % {{\<lambda>st. P st \<and> gs_getpath f' st = Some p}} s {{\<lambda>st. Q st \<and> (\<lambda> x . True) st}}"
+    using Hoare.VandI[OF H H'] unfolding H0
+    by auto
+
+  show "|! f' !| !% {!\<lambda>st. P st \<and> gs_getpath f' st = Some p!} prog {!Q'!}"
+    using vtsm_lift_cont[OF H0, of "(\<lambda> st . P st \<and> gs_getpath f' st = Some p)" p,
+                         OF _ Hp, of Q Q']
+    using Combine Hrec unfolding H0
+    by(auto)
+qed
+
+
+
+(* i think now we need more rules to deal with context.
+   for instance, describing partial executions (?)
+*)
+
+(*we need a way to relate sub-trees to entire trees.
+  this means we probably need some kind of actual lifting for the child-path
+
+*)
+
+(* we need a way to constrain P and Q's ability to talk about the path
+   substitution?
+   have path as another parameter?
+   maybe we can get away with just AND-ing
+*)
+
+(* sub-prog *)
+
+(* idea: sub program at path p1 in prog1
+   same sub program at path p2 in prog2
+
+   {{P \<and> path = p1}} prog1 {{Q \<and> halt}}
+   {{P \<and> path = p2}} prog2 {{Q \<and> halt}}
+   
+*)
+
+(*
+
+we also need a non-halting version; what would that look like?
+(or - halt in small program but not big)
+
+this only works if the small program halts from reaching top
+can we distinguish that case?
+
+
+
+*)
+lemma vtsm_ctx :
+  assumes H1 : "gs_sem f'1 = f"
+  assumes H2 : "gs_sem f'2 = f"
+  assumes Hp : "gensyn_get prog1 p = Some prog2"
+  assumes Exc1' : "|! f'1 !| % {{(\<lambda> st . P st \<and> gs_getpath f'1 st = p}} 
+                               prog1
+                               {{(\<lambda> st . gs_getpath f'1 st = None)}}"
+  assumes Exc2 : "|! f'2 !| % {{(\<lambda> st . P st \<and> gs_getpath f'2 st = Some []}} 
+                              prog2
+                              {{Q}}"
+  assumes Halt1 : "|! f'1 !| % {{(\<lambda> st . P st \<and> gs_getpath f'1 st = p}} 
+                              prog1
+                              {{(\<lambda> st . gs_getpath f'1 st = None)}}"
+
+  shows Exc1 : "|! f'1 !| % {{(\<lambda> st . P st \<and> gs_getpath f'1 st = p}} 
+                              prog1
+                              {{Q}}"
+ 
+
+  (*assumes Hp2 : "gensyn_get x1 p = Some x2"*)
+  
+  assumes Hstart1 : "\<And> st . P st \<Longrightarrow> gs_getpath f' st = Some p"
+  
+(* then we need a non-halting version of this *)
+
+(* OK, so new plan.
+- start with seq
+- relate behavior of sequence to individual ones using Hoare rules
+*)
 
 (*
  * mstate \<Rightarrow> childpath? just childpath?
